src/program_proof/mvcc/txn_acquire.v
@@ -3,11 +3,11 @@ From Perennial.program_proof.mvcc Require Import txn_common.
 Section program.
 Context `{!heapGS Σ, !mvcc_ghostG Σ}.
 
-Theorem wp_txn__acquire txn γ τ :
-  {{{ own_txn txn γ τ }}}
+Theorem wp_txn__acquire txn tid γ τ :
+  {{{ own_txn txn tid γ τ }}}
     Txn__acquire #txn
   {{{ (ok : bool), RET #ok;
-      if ok then own_txn_ready txn γ τ else own_txn txn γ τ
+      if ok then own_txn_ready txn tid γ τ else own_txn txn tid γ τ
   }}}.
 Admitted.
 
