src/program_proof/mvcc/txn_delete.v
@@ -6,11 +6,11 @@ Context `{!heapGS Σ, !mvcc_ghostG Σ}.
 (*****************************************************************)
 (* func (txn *Txn) Delete(key uint64) bool                       *)
 (*****************************************************************)
-Theorem wp_txn__Delete txn (k : u64) dbv γ τ :
-  {{{ own_txn txn γ τ ∗ txnmap_ptsto τ k dbv }}}
+Theorem wp_txn__Delete txn tid (k : u64) dbv γ τ :
+  {{{ own_txn txn tid γ τ ∗ txnmap_ptsto τ k dbv }}}
     Txn__Delete #txn #k
   {{{ (ok : bool), RET #ok;
-      own_txn txn γ τ ∗ txnmap_ptsto τ k Nil
+      own_txn txn tid γ τ ∗ txnmap_ptsto τ k Nil
   }}}.
 Proof.
   iIntros (Φ) "[Htxn Hptsto] HΦ".
@@ -38,7 +38,7 @@ Proof.
   { unfold own_txn.
     rewrite insert_union_l.
     set mods' := (<[ _ := _ ]> mods).
-    iExists _, view, mods'.
+    iExists view, mods'.
     eauto 20 with iFrame.
   }
   iFrame.
